candle/standard/syntax/littleTheoriesSyntaxNewSystemScript.sml
@@ -14,8 +14,8 @@ val _ = monadsyntax.enable_monad("error");
 
 fun rC q = rename [q] >> Cases_on q >> simp[]
 
-val cpn_distinct = TypeBase.distinct_of ``:ordering``
-val cpn_nchotomy = TypeBase.nchotomy_of ``:ordering``
+val cpn_distinct = TypeBase.distinct_of “:ordering”
+val cpn_nchotomy = TypeBase.nchotomy_of “:ordering”
 
 val strip_d1 = CONV_TAC (REWR_CONV (DECIDE “p ∨ q ⇔ ¬p ⇒ q”)) THEN strip_tac
 val strip_d2 = CONV_TAC (REWR_CONV (DECIDE “p ∨ q ⇔ ¬q ⇒ p”)) THEN strip_tac
@@ -27,44 +27,6 @@ Proof
   Induct_on ‘tm’ >> rw[term_ok'_def, term_ok_def]
 QED
 
-
-Theorem esubst_has_type_bool_alt:
-  ∀tm.
-    esubsts_ok (thy.ctys, thy.ctms) σ ∧
-    term_ok' thy tm ∧
-    theory_ok' thy ∧
-    tm has_type Bool ⇒
-    esubst σ avds tm has_type Bool
-Proof
-  rpt strip_tac >> irule esubst_has_type_bool
-  >> rw[] >> first_x_assum $ irule_at Any
-  >> simp[term_ok'_imp_term_ok]
-  >> qexists ‘thy.axs’
-  >> gvs[theory_ok_def, theory_ok'_def, ctys_def, ctms_def]
-  >> rw[FRANGE_FUNION]
-  >> metis_tac[is_std_sig_funion, sigof'_def,
-               term_ok_weakening, type_ok_weakening]
-QED
-
-
-Theorem proves_imp_proves':
-  ∀h. (thy, h) |- c ⇒ (lift_thy thy, {}, h) |-' c
-Proof
-  Induct_on ‘$|-’ >> rw[]
-  >- (irule proves'_ABS >> rw[])
-  >- (irule proves'_ASSUME >> rw[])
-  >- (irule proves'_BETA >> rw[])
-  >- (dxrule_all_then (ACCEPT_TAC o SRULE[]) proves'_DEDUCT_ANTISYM)
-  >- (dxrule_all proves'_EQ_MP >> rw[])
-  >- (irule proves'_INST >> rw[])
-  >- (irule proves'_INST_TYPE >> rw[])
-  >- (drule_all welltyped_comb >> strip_tac
-      >> dxrule_all proves'_MK_COMB >> simp[])
-  >- (irule proves'_REFL >> rw[])
-  >- (irule proves'_axioms >> rw[])
-QED
-
-
 Theorem theory_ok_drop_thy:
   ∀es. theory_ok' thy ∧ (∀a. a ∈ es ⇒ term_ok thy.sig a ∧ a has_type Bool) ⇒
        theory_ok (drop_thy es thy)
@@ -72,6 +34,7 @@ Proof
   rw[theory_ok'_def, theory_ok_def, drop_thy]
   >> gvs[ctys_def, ctms_def, sigof'_def, FRANGE_FUNION,
          type_ok_weakening, term_ok_weakening, is_std_sig_funion]
+  >> metis_tac[term_ok'_imp_term_ok, term_ok_weakening, ctys_def, ctms_def]
 QED
 
 Theorem term_ok_imp_term_ok':
@@ -88,6 +51,22 @@ Proof
   >> gvs[ctys_def, ctms_def, sigof'_def, FRANGE_FUNION,
          type_ok_weakening, term_ok_weakening, is_std_sig_funion]
   >> metis_tac[term_ok'_imp_term_ok, ctys_def, ctms_def]
+QED
+
+Theorem esubst_has_type_bool_alt:
+  ∀tm.
+    esubsts_ok (thy.ctys, thy.ctms) σ ∧
+    term_ok' thy tm ∧
+    theory_ok' thy ∧
+    tm has_type Bool ⇒
+    esubst σ avds tm has_type Bool
+Proof
+  rw[] >> irule esubst_has_type_bool
+  >> conj_asm1_tac >- simp[]
+  >> qexistsl_tac [`(thy:ethy).axs`, `((thy:ethy).ctys, thy.ctms)`]
+  >> simp[term_ok'_imp_term_ok]
+  >> qspec_then `{}` mp_tac theory_ok_drop_thy_alt
+  >> simp[drop_thy]
 QED
 
 Theorem ty_esubst_type_ok:
@@ -111,10 +90,287 @@ Proof
   >> metis_tac[]
 QED
 
+Theorem ty_esubst_type_ok_id:
+  ∀ty σ. type_ok tys ty ∧ DISJOINT (FDOM (FST σ)) (FDOM tys) ⇒ ty_esubst σ ty = ty
+Proof
+  ho_match_mp_tac type_ind >> rw[]
+  >- simp[ty_esubst_def]
+  >> Cases_on `l : type list` >> simp[ty_esubst_def]
+  >- (CASE_TAC >> gvs[type_ok_def, FLOOKUP_DEF, IN_DISJOINT] >> metis_tac[])
+  >> gvs[type_ok_def, EVERY_MEM, MAP_EQ_ID] >> metis_tac[]
+QED
+
+Theorem VFREE_IN_esubst_iff:
+  esubsts_ok sig σ ∧ term_ok sig tm ⇒
+  (VFREE_IN (Var u uty) (esubst σ [] tm) ⇔
+   ∃oty. VFREE_IN (Var u oty) tm ∧ uty = ty_esubst σ oty)
+Proof
+  rw[esubst_def, esubst_ty_def]
+  >> `∃tm1. esubst_ty0 [] σ [] tm = return tm1`
+    by metis_tac[esubst_ty0_always_returns]
+  >> simp[]
+  >> `VFREE_IN (Var u uty) (esubst_tm σ tm1) ⇔ VFREE_IN (Var u uty) tm1`
+    by metis_tac[VFREE_IN_esubst_tm]
+  >> simp[]
+  >> irule esubst_ty0_all_free
+  >> rpt $ first_assum $ irule_at Any >> simp[MEM]
+QED
+
+Theorem axioms_ok_esubst:
+  axioms_ok axs ∧ (∀p. p ∈ axs ⇒ term_ok sig p) ∧ esubsts_ok sig σ ⇒
+  axioms_ok (IMAGE (esubst σ []) axs)
+Proof
+  rw[axioms_ok_def, PULL_EXISTS]
+  >> `∀u uty. VFREE_IN (Var u uty) (esubst σ [] x) ⇔
+              ∃oty. VFREE_IN (Var u oty) x ∧ uty = ty_esubst σ oty`
+    by (irule VFREE_IN_esubst_iff >> metis_tac[])
+  >> gvs[] >> metis_tac[]
+QED
+
+Theorem DISJOINT_FLOOKUP:
+  DISJOINT (FDOM f1) (FDOM f2) ∧ FLOOKUP f1 k = SOME v ⇒ FLOOKUP f2 k = NONE
+Proof
+  rw[] >> imp_res_tac $ iffRL FDOM_FLOOKUP >> irule $ iffRL $ cj 1 flookup_thm >> ASM_SET_TAC[]
+QED
+
+Theorem SUBMAP_FUNION_mono_r':
+  g1 ⊑ g2 ⇒ f ⊌ g1 ⊑ f ⊌ g2
+Proof
+  rw[SUBMAP_DEF, FUNION_DEF, FDOM_FUNION] >> metis_tac[]
+QED
+
+Theorem esubsts_ok'_esubsts_ok:
+  esubsts_ok' thy σ ∧ theory_ok' thy ⇒ esubsts_ok (thy.ctys, thy.ctms) σ
+Proof
+  Cases_on `σ` >> rename1`(σ,θ)` >> rw[esubsts_ok'_def, esubsts_ok_def, theory_ok'_def]
+  >- (first_x_assum drule >> simp[ctms_def, FLOOKUP_FUNION] >> CASE_TAC >> rw[]
+      >> drule_all DISJOINT_FLOOKUP >> simp[])
+  >> first_x_assum drule >> rw[] >> gvs[term_ok_def, term_ok'_def]
+  >> gvs[ctys_def, type_ok_weakening, ctms_def, esubst_thy_def, FLOOKUP_FUNION]
+  >> qexists `ty0` >> gvs[monomorphic_type_subst] >> rw[FLOOKUP_o_f]
+  >> gvs[ctys_def, type_ok_weakening, ctms_def, esubst_thy_def, FLOOKUP_FUNION, AllCaseEqs(),
+         FLOOKUP_o_f]
+  >> gvs[FLOOKUP_o_f, FLOOKUP_FUNION, AllCaseEqs()]
+  >- (gvs[FLOOKUP_FDIFF] >> metis_tac[])
+  >- (irule ty_esubst_type_ok_id >> qexists_tac `(thy:ethy).tys` >> simp[]
+      >> conj_tac >- metis_tac[DISJOINT_SUBSET, DISJOINT_SYM]
+      >> first_x_assum irule >> simp[IN_FRANGE_FLOOKUP] >> metis_tac[])
+  >> `(thy.tys ⊌ FDIFF thy.etys (FDOM σ)) ⊑ (thy.tys ⊌ thy.etys)` by
+       (irule SUBMAP_FUNION_mono_r' >> simp[FDIFF_def, SUBMAP_DRESTRICT])
+  >> imp_res_tac type_ok_extend
+  >> rw[] >> metis_tac[]
+QED
+
+Theorem type_ok_restrict_nullary:
+  ∀ty. type_ok (tys ⊌ etys) ty ∧
+       DISJOINT (FDOM tys) (FDOM etys) ∧
+       FRANGE etys ⊆ {0} ∧
+       DISJOINT ss (nullary_ops_of ty) ∧
+       ss ⊆ FDOM etys ⇒
+       type_ok (tys ⊌ FDIFF etys ss) ty
+Proof
+  ho_match_mp_tac type_ind >> rw[]
+  >- simp[type_ok_def]
+  >> rpt strip_tac
+  >> Cases_on `l` >> gvs[type_ok_def, nullary_ops_of_def]
+  >- (gvs[FLOOKUP_FUNION, AllCaseEqs()]
+      >> simp[FLOOKUP_FDIFF])
+  >> simp[type_ok_def] >> rpt conj_tac
+  >- (gvs[type_ok_def, FLOOKUP_FUNION, AllCaseEqs()]
+      >> `SUC (LENGTH t) ∈ FRANGE etys`
+           by (simp[IN_FRANGE_FLOOKUP] >> metis_tac[])
+      >> fs[SUBSET_DEF] >> res_tac >> fs[])
+  >- (rpt strip_tac >> first_x_assum irule
+      >> gvs[IN_DISJOINT] >> metis_tac[])
+  >> simp[EVERY_MEM] >> rpt strip_tac
+  >> gvs[EVERY_MEM]
+  >> first_x_assum drule >> strip_tac
+  >> first_x_assum irule
+  >> gvs[IN_DISJOINT, MEM_MAP] >> metis_tac[]
+QED
+
+Theorem esubsts_ok'_frange_type_ok:                                                    
+  theory_ok' thy ∧ esubsts_ok' thy (σty, σtm) ∧ ty ∈ FRANGE σty ⇒
+  type_ok (esubst_thy (σty, σtm) thy).ctys ty
+Proof
+  rw[theory_ok'_def, esubsts_ok'_def, ctys_def, esubst_thy_def] >> res_tac
+  >> irule type_ok_restrict_nullary >> simp[]
+QED
+
+Theorem ty_esubst_type_ok':
+  theory_ok' thy ∧ esubsts_ok' thy σ ∧ type_ok thy.ctys ty ⇒
+  type_ok (esubst_thy σ thy).ctys (ty_esubst σ ty)
+Proof
+  strip_tac
+  >> drule_all esubsts_ok'_esubsts_ok >> strip_tac
+  >> ntac 2 (pop_assum mp_tac) >> qid_spec_tac `ty`
+  >> Induct_on `ty` using type_ind >> rw[]
+  >- simp[ty_esubst_def, type_ok_def]
+  >> Cases_on `σ` >> rename1 `(σty, σtm)`
+  >> Cases_on `l`
+  >- (rw[ty_esubst_def] >> CASE_TAC
+      >- (rw[type_ok_def, esubst_thy_def, ctys_def, FLOOKUP_FUNION]
+          >> gvs[type_ok_def, ctys_def, FLOOKUP_FUNION, AllCaseEqs()]
+          >> gvs[esubsts_ok_def, SUBSET_DEF, FDOM_FLOOKUP, FLOOKUP_FDIFF])
+      >> rename1 `FLOOKUP σty m = SOME x`
+      >> gvs[esubst_thy_def, ctys_def, esubsts_ok_def]
+      >> drule_then drule esubsts_ok'_frange_type_ok >> disch_then $ qspec_then ‘x’ mp_tac
+      >> simp[IN_FRANGE_FLOOKUP, SF SFY_ss, esubst_thy_def, ctys_def])
+  >> `FLOOKUP thy.tys m = SOME (SUC (LENGTH t))`
+       by (gvs[type_ok_def, ctys_def, FLOOKUP_FUNION, AllCaseEqs()]
+           >> `SUC (LENGTH t) ∈ FRANGE thy.etys`
+                by (simp[IN_FRANGE_FLOOKUP] >> metis_tac[])
+           >> fs[theory_ok'_def, SUBSET_DEF] >> res_tac >> gvs[])
+  >> rw[ty_esubst_def, type_ok_def, EVERY_MEM, MEM_MAP, PULL_EXISTS]
+  >- simp[esubst_thy_def, ctys_def, FLOOKUP_FUNION, FDOM_FLOOKUP]
+  >> first_x_assum (irule o BETA_RULE o REWRITE_RULE [EVERY_MEM]) >> simp[]
+  >> gvs[type_ok_def, ctys_def, EVERY_MEM]
+QED
+
+Theorem esubst_thy_ctms_preserved:
+  theory_ok' thy ∧ esubsts_ok' thy (σty, σtm) ∧
+  FLOOKUP thy.ctms n = SOME ty0 ∧ n ∉ FDOM σtm ⇒
+  FLOOKUP (esubst_thy (σty, σtm) thy).ctms n = SOME (ty_esubst (σty, σtm) ty0)
+Proof
+  strip_tac
+  >> simp[esubst_thy_def, ctms_def, FLOOKUP_FUNION, FLOOKUP_o_f, FLOOKUP_FDIFF]
+  >> Cases_on `FLOOKUP thy.tms n`
+  >- (gvs[ctms_def, FLOOKUP_FUNION])
+  >> `x = ty0` by gvs[ctms_def, FLOOKUP_FUNION]
+  >> gvs[]
+  >> `ty_esubst (σty,σtm) ty0 = ty0` by
+       (irule ty_esubst_type_ok_id >> qexists `thy.tys`
+        >> gvs[theory_ok'_def, esubsts_ok'_def]
+        >> conj_tac
+        >- metis_tac[DISJOINT_SUBSET, DISJOINT_SYM]
+        >> first_x_assum irule >> simp[IN_FRANGE_FLOOKUP] >> metis_tac[])
+  >> simp[]
+QED
+
+Theorem term_ok'_vsubst_variant:
+  term_ok' thy tm ∧ type_ok thy.ctys ty ⇒
+  term_ok' thy (VSUBST [(Var x1 ty, Var x2 ty)] tm)
+Proof
+  rw[]
+  >> irule term_ok_imp_term_ok'
+  >> irule term_ok_VSUBST
+  >> simp[term_ok'_imp_term_ok, term_ok_def]
+QED
+
+Theorem esubst_ty0_tm_ok':
+  ∀env σ avds tm subst_tm.
+    esubst_ty0 env σ avds tm = return subst_tm ∧
+    term_ok' thy tm ∧ theory_ok' thy ∧ esubsts_ok' thy σ ∧ esubsts_ok (thy.ctys, thy.ctms) σ ∧
+    (∀v1 v2. MEM (v1, v2) env ⇒ ∃n ty. v1 = Var n ty ∧ v2 = Var n (ty_esubst σ ty)) ⇒
+    term_ok' (esubst_thy σ thy) (esubst_tm σ subst_tm)
+Proof
+  recInduct esubst_ty0_ind >> rw[]
+  (* Var *)
+  >- (gvs[esubst_ty0_def, AllCaseEqs()]
+      >> simp[esubst_tm_def, term_ok'_def]
+      >> irule ty_esubst_type_ok' >> gvs[term_ok'_def] >> metis_tac[])
+  (* Const *)
+  >- (gvs[esubst_ty0_def, term_ok'_def]
+      >> Cases_on `σ` >> rename1 `(σty, σtm)`
+      >> simp[esubst_tm_def]
+      >> Cases_on `FLOOKUP σtm n`
+      >- (simp[term_ok'_def]
+          >> qexists `ty_esubst (σty, σtm) ty0`
+          >> rpt conj_tac
+          >- (irule esubst_thy_ctms_preserved >> simp[]
+              >> strip_tac >> gvs[FDOM_FLOOKUP])
+          >- (irule ty_esubst_type_ok' >> metis_tac[])
+          >> metis_tac[ty_esubst_TYPE_SUBST])
+      >> (rename1 `FLOOKUP σtm n = SOME repl`
+          >> gvs[esubsts_ok'_def]
+          >> `repl ∈ FRANGE σtm` by (simp[IN_FRANGE_FLOOKUP] >> metis_tac[])
+          >> res_tac >> gvs[]))
+  (* Comb *)
+  >- (gvs[esubst_ty0_def, bind_EQ_return, term_ok'_def]
+      >> simp[esubst_tm_def, term_ok'_def]
+      >> rpt conj_tac
+      >- metis_tac[term_ok'_imp_term_ok, term_ok_welltyped]
+      >- metis_tac[term_ok'_imp_term_ok, term_ok_welltyped]
+      >> Cases_on `σ` >> rename1 `(σty, σtm)`
+      >> metis_tac[typeof_esubst_ty, typeof_esubst_tm_esubst_ty0,
+                   term_ok'_imp_term_ok, ty_esubst_fun])
+  (* Abs *)
+  >> gvs[term_ok'_def, esubst_ty0_def, bind_EQ_return, bind_EQ_error, try_eq_return]
+  >- (simp[esubst_tm_def, term_ok'_def]
+      >> rpt conj_tac
+      >- (irule ty_esubst_type_ok' >> metis_tac[])
+      >> first_x_assum irule >> simp[] >> metis_tac[])
+  >> gvs[AllCaseEqs(), bind_EQ_return]
+  >> simp[esubst_tm_def, term_ok'_def]
+  >> rw[]
+  >- (irule ty_esubst_type_ok' >> metis_tac[])
+  >> first_x_assum irule >> qexists `body1`
+  >> rw[]
+  >- metis_tac[]
+  >> irule term_ok'_vsubst_variant
+  >> simp[]
+QED
+
+Theorem esubst_term_ok':
+  theory_ok' thy ∧ esubsts_ok' thy σ ∧ term_ok' thy tm ⇒
+  term_ok' (esubst_thy σ thy) (esubst σ avds tm)
+Proof
+  strip_tac
+  >> drule_all esubsts_ok'_esubsts_ok >> strip_tac
+  >> simp[esubst_def, esubst_ty_def]
+  >> `∃tm1. esubst_ty0 [] σ avds tm = return tm1`
+       by metis_tac[esubst_ty0_always_returns, term_ok'_imp_term_ok]
+  >> simp[]
+  >> irule esubst_ty0_tm_ok'
+  >> simp[] >> metis_tac[MEM]
+QED
+
+Theorem frange_esubst_thy_etms:
+  ty ∈ FRANGE (esubst_thy σ thy).etms ⇒
+  ∃ty0. ty = ty_esubst σ ty0 ∧ ty0 ∈ FRANGE thy.etms
+Proof
+  simp[esubst_thy_def, IN_FRANGE_FLOOKUP, FLOOKUP_o_f, FLOOKUP_FDIFF]
+  >> strip_tac >> every_case_tac >> gvs[]
+  >> simp[IN_FRANGE_FLOOKUP] >> metis_tac[]
+QED
+
 Theorem theory_ok'_esubst:
   theory_ok' thy ∧ esubsts_ok' thy σ ⇒ theory_ok' (esubst_thy σ thy)
 Proof
-  cheat
+  strip_tac
+  >> simp[theory_ok'_def, sigof'_def]
+  >> rpt conj_tac
+  >- (simp[esubst_thy_def] >> gvs[theory_ok'_def])
+  >- (rw[] >> drule frange_esubst_thy_etms >> strip_tac >> gvs[]
+      >> irule ty_esubst_type_ok' >> simp[]
+      >> gvs[theory_ok'_def])
+  >- (simp[esubst_thy_def] >> gvs[theory_ok'_def, FDIFF_def, FDOM_DRESTRICT] >> ASM_SET_TAC[])
+  >- (simp[esubst_thy_def] >> gvs[theory_ok'_def, FDIFF_def, FDOM_DRESTRICT] >> ASM_SET_TAC[])
+  >- (rpt strip_tac
+      >> `∃x. p = esubst σ [] x ∧ x ∈ thy.axs` by (fs[esubst_thy_def] >> metis_tac[])
+      >> gvs[]
+      >> drule_all esubsts_ok'_esubsts_ok >> strip_tac
+      >- (irule esubst_term_ok' >> gvs[theory_ok'_def])
+      >> irule esubst_has_type_bool_alt
+         >> first_assum $ irule_at Any >> gvs[theory_ok'_def])
+  >- (rpt strip_tac
+      >> `∃x. p = esubst σ [] x ∧ x ∈ thy.eaxs` by (fs[esubst_thy_def] >> metis_tac[])
+      >> gvs[]
+      >> drule_all esubsts_ok'_esubsts_ok >> strip_tac
+      >- (irule esubst_term_ok' >> gvs[theory_ok'_def])
+      >> irule esubst_has_type_bool_alt
+         >> first_assum $ irule_at Any >> gvs[theory_ok'_def])
+  >- (simp[esubst_thy_def] >> gvs[theory_ok'_def, sigof'_def])
+  >- (drule_all esubsts_ok'_esubsts_ok >> strip_tac
+      >> simp[esubst_thy_def]
+      >> irule axioms_ok_esubst >> first_assum $ irule_at Any
+      >> gvs[theory_ok'_def] >> metis_tac[term_ok'_imp_term_ok])
+  >- (drule_all esubsts_ok'_esubsts_ok >> strip_tac
+      >> simp[esubst_thy_def]
+      >> irule axioms_ok_esubst >> first_assum $ irule_at Any
+      >> gvs[theory_ok'_def] >> metis_tac[term_ok'_imp_term_ok])
+  >> simp[esubst_thy_def]
+  >> simp[FDIFF_def] >> metis_tac[theory_ok'_def, SUBSET_TRANS, FRANGE_DRESTRICT_SUBSET]
 QED
 
 Theorem proves'_imp_theory_ok':
@@ -140,33 +396,65 @@ Proof
   >> gvs[ctys_def, ctms_def] >> first_assum $ irule_at Any >> ASM_SET_TAC[]
 QED
 
-Theorem DISJOINT_FLOOKUP:
-  DISJOINT (FDOM f1) (FDOM f2) ∧ FLOOKUP f1 k = SOME v ⇒ FLOOKUP f2 k = NONE
-Proof
-  rw[] >> imp_res_tac $ iffRL FDOM_FLOOKUP >> irule $ iffRL $ cj 1 flookup_thm >> ASM_SET_TAC[]
-QED
-
-Theorem esubsts_ok'_esubsts_ok:
-  esubsts_ok' thy σ ∧ theory_ok' thy ⇒ esubsts_ok (thy.ctys, thy.ctms) σ
-Proof
-  Cases_on ‘σ’ >> rename1‘(σ,θ)’ >> rw[esubsts_ok'_def, esubsts_ok_def, theory_ok'_def]
-  >- (first_x_assum drule >> simp[ctms_def, FLOOKUP_FUNION] >> CASE_TAC >> rw[]
-      >> drule_all DISJOINT_FLOOKUP >> simp[])
-  >> first_x_assum drule >> rw[] >> gvs[term_ok_def, term_ok'_def]
-  >> gvs[ctys_def, type_ok_weakening, ctms_def, esubst_thy_def, FLOOKUP_FUNION]
-  >> qexists ‘ty0’ >> gvs[monomorphic_type_subst] >> rw[FLOOKUP_o_f]
-  >> gvs[ctys_def, type_ok_weakening, ctms_def, esubst_thy_def, FLOOKUP_FUNION, AllCaseEqs()]
-  >> cheat
-QED
-
 val contrapos_tac = CONV_TAC (REWR_CONV (DECIDE “p ⇒ q ⇔ ¬q ⇒ ¬p”)) THEN strip_tac
 
 Theorem ty_esubst_o_f_thy_tms:
   ∀thy. theory_ok' thy ∧ esubsts_ok' thy σ ⇒ ty_esubst σ o_f thy.tms = thy.tms
 Proof
-  cheat
+  rw[theory_ok'_def] >> Cases_on `σ` >> gvs[esubsts_ok'_def]
+  >> simp[fmap_eq_flookup, FLOOKUP_o_f]
+  >> rw[] >> CASE_TAC >> simp[]
+  >> irule ty_esubst_type_ok_id
+  >> qexists_tac `(thy:ethy).tys` >> simp[]
+  >> conj_tac
+  >- metis_tac[DISJOINT_SUBSET, DISJOINT_SYM]
+  >> first_x_assum irule >> simp[IN_FRANGE_FLOOKUP] >> metis_tac[]
 QED
 
+Theorem axioms_ok_no_var_collapse:
+  axioms_ok axs ⇒ ∀σ ax. ax ∈ axs ⇒ no_var_collapse σ ax
+Proof
+  rw[axioms_ok_def, no_var_collapse] >> res_tac
+QED
+
+Theorem proves_esubst_drop_thy:
+  (drop_thy es thy, h) |- c ∧
+  theory_ok' thy ∧
+  esubsts_ok' thy σ ∧
+  (∀ax. ax ∈ es ⇒ no_var_collapse σ ax) ⇒
+  (drop_thy (IMAGE (esubst σ []) es) (esubst_thy σ thy),
+   term_image (esubst σ []) h) |- esubst σ (FLAT (MAP tm_names h)) c
+Proof
+  rw[drop_thy] >> drule_at (Pat ‘_ |- _’) proves_substitutable
+  >> disch_then $ qspec_then ‘σ’ mp_tac >> impl_tac
+  >- (conj_tac >- metis_tac[proves_theory_ok]
+      >> conj_tac >- metis_tac[esubsts_ok'_esubsts_ok]
+      >> fs[theory_ok'_def] >> imp_res_tac axioms_ok_no_var_collapse
+      >> rw[] >> res_tac >> first_x_assum irule)
+  >> cheat
+QED
+
+Theorem proves_imp_proves':
+  ∀thy' h c. (thy', h) |- c ⇒
+    axioms_ok (axsof thy') ⇒ (lift_thy thy', {}, h) |-' c
+Proof
+  Induct_on `$|-` >> rw[] >> fs[]
+  >- (irule proves'_ABS >> simp[])
+  >- (irule proves'_ASSUME >> simp[term_ok_imp_term_ok'])
+  >- (irule proves'_BETA >> simp[term_ok_imp_term_ok'])
+  >- (rev_drule_then drule proves'_DEDUCT_ANTISYM >> simp[])
+  >- (drule_all proves'_EQ_MP >> simp[])
+  >- (irule proves'_INST >> simp[]
+      >> first_x_assum $ irule_at Any >> rw[]
+      >> first_x_assum drule >> rw[]
+      >> irule term_ok_imp_term_ok' >> simp[])
+  >- (irule proves'_INST_TYPE >> simp[])
+  >- (rev_drule_then drule proves'_MK_COMB >> simp[])
+  >- (irule proves'_REFL >> simp[term_ok_imp_term_ok'])
+  >> irule proves'_axioms >> simp[]
+QED
+
+        
 Theorem proves'_imp_proves:
   ∀thy' c h used_eaxs.
     (thy', used_eaxs, h) |-' c ⇒ (drop_thy used_eaxs thy', h) |- c
@@ -178,7 +466,7 @@ Proof
   >- (irule proves_DEDUCT_ANTISYM >> conj_tac >> irule drop_thy_weakening
       >> imp_res_tac proves_theory_ok >> gvs[theory_ok_def, drop_thy]
       >> (conj_tac >- metis_tac[term_ok'_imp_term_ok]
-          >> first_x_assum $ irule_at Any >> simp[]))
+          >> metis_tac[SUBSET_UNION]))
   >- (irule proves_EQ_MP
       >> imp_res_tac proves_theory_ok >> gvs[theory_ok_def, drop_thy]
       >> first_x_assum $ irule_at Any >> simp[]
@@ -207,15 +495,266 @@ Proof
                           ‘h2’, ‘c’, ‘c'’]
                          assume_tac axioms_eliminable
           >> gvs[]))
-  >- (gvs[drop_thy] >> drule proves_theory_ok >> drule esubsts_ok'_esubsts_ok >> rw[]
-      >> ‘∀tm. MEM tm h ∨ tm = c ⇒ no_var_collapse σ tm’ by metis_tac[]
-      >> drule_all proves_substitutable >> rw[esubst_thy_def, esubst_sig_def, ctms_def, ctys_def, o_f_FUNION]
-      >> gvs[ty_esubst_o_f_thy_tms] >> imp_res_tac proves_theory_ok >> irule axiom_weakening
-      >> first_x_assum $ irule_at Any >> gvs[theory_ok'_def] >> rw[SUBSET_DEF, DISJ_IMP_THM]
-      >> cheat)
+  >- (
+    drule proves'_imp_theory_ok' >> strip_tac
+    >> irule proves_esubst_drop_thy >> metis_tac[])
   >- (irule proves_axioms >> rw[]
       >- (irule theory_ok_drop_thy_alt >> gvs[theory_ok'_def])
       >> rw[drop_thy])
+QED
+
+Theorem extends'_ind:
+  ∀P. (∀upd ctxt. upd updates' ctxt ∧ P ctxt ⇒ P (upd::ctxt)) ⇒
+    ∀ctxt1 ctxt2. ctxt2 extends' ctxt1 ⇒ P ctxt1 ⇒ P ctxt2
+Proof
+  gen_tac >> strip_tac >>
+  simp[extends'_def] >>
+  CONV_TAC SWAP_FORALL_CONV >>
+  ho_match_mp_tac RTC_INDUCT >>
+  rw[] >> first_x_assum match_mp_tac >>
+  rw[]
+QED
+
+Theorem REV_ASSOCD_const_subst:
+  ∀l y ty d.
+    MEM (y, ty) (MAP (λ(s,t). (s, typeof t)) l) ⇒
+    ∃nm. REV_ASSOCD (Var y ty)
+           (MAP (λ(s,t'). (Const s (typeof t'), Var s (typeof t'))) l) d
+         = Const nm ty
+Proof
+  Induct >> rw[REV_ASSOCD] >> PairCases_on `h` >> fs[REV_ASSOCD]
+  >> Cases_on `h0 = y ∧ typeof h1 = ty` >> fs[]
+  >> first_x_assum drule >> rw[]
+QED
+
+Theorem extends_axioms_ok:
+  ∀ctxt1 ctxt2. ctxt2 extends ctxt1 ⇒ axioms_ok (axsof ctxt1) ⇒ axioms_ok (axsof ctxt2)
+Proof
+  ho_match_mp_tac extends_ind >> Cases >> rw[axioms_ok_def] >> res_tac >> gvs[conexts_of_upd_def]
+  >- (gvs[conexts_of_upd_def, VFREE_IN_def, Once updates_cases] >> ntac 2 $ pop_assum mp_tac
+      >> DEP_REWRITE_TAC[VFREE_IN_VSUBST] >> rw[]
+      >- (dxrule proves_term_ok >> simp[EVERY_MEM, term_ok_welltyped, SF SFY_ss])
+      >> res_tac >> rev_dxrule REV_ASSOCD_const_subst >> disch_then $ qspec_then ‘Var y' ty'’ mp_tac
+      >> rw[] >> fs[VFREE_IN_def])
+  >> gvs[VFREE_IN_def, equation_def, Once updates_cases, CLOSED_def]
+QED
+
+Theorem init_axioms_ok:
+  axioms_ok (axsof init_ctxt)
+Proof
+  simp[EVAL ``axsof init_ctxt``, axioms_ok_def]
+QED
+
+Theorem SUBMAP_FUNION_mono:
+  f1 ⊑ f2 ∧ DISJOINT (FDOM f2) (FDOM g) ⇒ f1 ⊌ g ⊑ f2 ⊌ g
+Proof
+  rw[SUBMAP_DEF, FUNION_DEF, FDOM_FUNION, FAPPLY_FUPDATE_THM] >>
+  metis_tac[IN_DISJOINT]
+QED
+
+Theorem SUBMAP_FUNION_mono_r:
+  g1 ⊑ g2 ⇒ f ⊌ g1 ⊑ f ⊌ g2
+Proof
+  rw[SUBMAP_DEF, FUNION_DEF, FDOM_FUNION] >> metis_tac[]
+QED
+
+Theorem term_ok'_sig_eq:
+  ∀tm thy1 thy2. thy1.ctys = thy2.ctys ∧ thy1.ctms = thy2.ctms ⇒
+       (term_ok' thy1 tm ⇔ term_ok' thy2 tm)
+Proof
+  Induct_on `tm` >> simp[term_ok'_def] >> metis_tac[]
+QED
+
+Theorem term_ok'_extend:
+  ∀tm thy1 thy2. thy1.ctys ⊑ thy2.ctys ∧ thy1.ctms ⊑ thy2.ctms ∧
+       term_ok' thy1 tm ⇒ term_ok' thy2 tm
+Proof
+  Induct_on `tm` >> rw[term_ok'_def] >>
+  metis_tac[type_ok_extend, SUBMAP_FLOOKUP_EQN]
+QED
+
+Theorem theory_ok'_ax_ext:
+  theory_ok'
+  <|tms := tms; tys := tys; axs := axs;
+    etms := etms; etys := etys; eaxs := eaxs|> ∧
+  (∀p. p ∈ axs1 ⇒ term_ok (tys, tms) p ∧ p has_type Bool) ∧
+  axioms_ok axs1 ⇒
+  theory_ok'
+  <|tms := tms; tys := tys; axs := axs1;
+    etms := etms; etys := etys; eaxs := eaxs|>
+Proof
+  strip_tac >> fs[theory_ok'_def, sigof'_def, ctys_def, ctms_def] >>
+  rpt conj_tac >> rpt strip_tac >> res_tac
+  >- (irule term_ok_term_ok'_weakening >> simp[sigof'_def])
+  >- (irule term_ok'_extend >>
+      qexists_tac `<|tms := tms; tys := tys; axs := axs;
+                     etms := etms; etys := etys; eaxs := eaxs|>` >>
+      simp[ctys_def, ctms_def, SUBMAP_REFL])
+QED
+
+Theorem theory_ok'_tms_extend:
+  theory_ok' <|tms := tms; tys := tys; axs := axs; etms := etms; etys := etys; eaxs := eaxs|> ∧
+  type_ok tys ty ∧ name ∉ FDOM tms ∧ name ∉ FDOM etms ⇒
+  theory_ok' <|tms := tms |+ (name, ty); tys := tys; axs := axs; etms := etms; etys := etys; eaxs := eaxs|>
+Proof
+  strip_tac >> fs[theory_ok'_def, sigof'_def, ctys_def, ctms_def] >>
+  `tms ⊌ etms ⊑ (tms |+ (name,ty)) ⊌ etms` by (
+    irule SUBMAP_FUNION_mono >>
+    simp[SUBMAP_FUPDATE_EXTENDED, FDOM_FUPDATE, DISJOINT_INSERT]) >>
+  rw[theory_ok'_def, sigof'_def, ctys_def, ctms_def] >>
+  rpt conj_tac >> rpt strip_tac
+  >- (gvs[FRANGE_FLOOKUP, FLOOKUP_UPDATE, AllCaseEqs()] >> res_tac)
+  >- (metis_tac[IN_FRANGE_DOMSUB_suff])
+  >- (res_tac >> irule term_ok'_extend >>
+      qexists_tac `<|tms := tms; tys := tys; axs := axs;
+                     etms := etms; etys := etys; eaxs := eaxs|>` >>
+      simp[ctys_def, ctms_def])
+  >- (res_tac >> irule term_ok'_extend >>
+      qexists_tac `<|tms := tms; tys := tys; axs := axs;
+                     etms := etms; etys := etys; eaxs := eaxs|>` >>
+      simp[ctys_def, ctms_def])
+  >- (irule is_std_sig_extend >>
+      metis_tac[SUBMAP_REFL, SUBMAP_FUPDATE_EXTENDED])
+QED
+
+Theorem theory_ok'_tys_extend:
+  theory_ok' <|tms := tms; tys := tys; axs := axs; etms := etms; etys := etys; eaxs := eaxs|> ∧
+  name ∉ FDOM tys ∧ name ∉ FDOM etys ⇒
+  theory_ok' <|tms := tms; tys := tys |+ (name, arity); axs := axs; etms := etms; etys := etys; eaxs := eaxs|>
+Proof
+  strip_tac >> fs[theory_ok'_def, sigof'_def, ctys_def, ctms_def] >>
+  `tys ⊌ etys ⊑ (tys |+ (name,arity)) ⊌ etys` by (
+    irule SUBMAP_FUNION_mono >>
+    simp[SUBMAP_FUPDATE_EXTENDED, FDOM_FUPDATE, DISJOINT_INSERT]) >>
+  rw[theory_ok'_def, sigof'_def, ctys_def, ctms_def] >>
+  rpt conj_tac >> rpt strip_tac
+  >- (res_tac >> irule type_ok_extend >> first_assum (irule_at Any) >>
+      simp[SUBMAP_FUPDATE_EXTENDED])
+  >- (res_tac >> irule type_ok_extend >> first_assum (irule_at Any) >> simp[])
+  >- (res_tac >> irule term_ok'_extend >>
+      qexists_tac `<|tms := tms; tys := tys; axs := axs;
+                     etms := etms; etys := etys; eaxs := eaxs|>` >>
+      simp[ctys_def, ctms_def])
+  >- (res_tac >> irule term_ok'_extend >>
+      qexists_tac `<|tms := tms; tys := tys; axs := axs;
+                     etms := etms; etys := etys; eaxs := eaxs|>` >>
+      simp[ctys_def, ctms_def])
+  >- (irule is_std_sig_extend >>
+      metis_tac[SUBMAP_REFL, SUBMAP_FUPDATE_EXTENDED])
+QED
+
+Theorem theory_ok'_etys_extend:
+  theory_ok' <|tms := tms; tys := tys; axs := axs; etms := etms; etys := etys; eaxs := eaxs|> ∧
+  name ∉ FDOM tys ∧ name ∉ FDOM etys ∧ arity = 0 ⇒
+  theory_ok' <|tms := tms; tys := tys; axs := axs; etms := etms; etys := etys |+ (name, arity); eaxs := eaxs|>
+Proof
+  strip_tac >> gvs[theory_ok'_def, sigof'_def, ctys_def, ctms_def] >>
+  `tys ⊌ etys ⊑ tys ⊌ (etys |+ (name,0))` by (
+    irule SUBMAP_FUNION_mono_r >> simp[SUBMAP_FUPDATE_EXTENDED]) >>
+  rw[theory_ok'_def, sigof'_def, ctys_def, ctms_def] >>
+  rpt conj_tac >> rpt strip_tac
+  >- (res_tac >> irule type_ok_extend >> first_assum (irule_at Any) >> simp[])
+  >- (res_tac >> irule term_ok'_extend >>
+      qexists_tac `<|tms := tms; tys := tys; axs := axs;
+                     etms := etms; etys := etys; eaxs := eaxs|>` >>
+      simp[ctys_def, ctms_def, SUBMAP_REFL])
+  >- (res_tac >> irule term_ok'_extend >>
+      qexists_tac `<|tms := tms; tys := tys; axs := axs;
+                     etms := etms; etys := etys; eaxs := eaxs|>` >>
+      simp[ctys_def, ctms_def, SUBMAP_REFL])
+  >> gvs[DOMSUB_NOT_IN_DOM, FRANGE_FUPDATE_DOMSUB, SUBSET_DEF]
+QED
+
+Theorem theory_ok'_etms_extend:
+  theory_ok' <|tms := tms; tys := tys; axs := axs; etms := etms; etys := etys; eaxs := eaxs|> ∧
+  type_ok (tys ⊌ etys) ty ∧ name ∉ FDOM tms ∧ name ∉ FDOM etms ⇒
+  theory_ok' <|tms := tms; tys := tys; axs := axs; etms := etms |+ (name, ty); etys := etys; eaxs := eaxs|>
+Proof
+  strip_tac >> fs[theory_ok'_def, sigof'_def, ctys_def, ctms_def] >>
+  `tms ⊌ etms ⊑ tms ⊌ (etms |+ (name,ty))` by (
+    irule SUBMAP_FUNION_mono_r >> simp[SUBMAP_FUPDATE_EXTENDED]) >>
+  rw[theory_ok'_def, sigof'_def, ctys_def, ctms_def] >>
+  rpt conj_tac >> rpt strip_tac
+  >- (gvs[FRANGE_FLOOKUP, FLOOKUP_UPDATE, AllCaseEqs()] >> res_tac)
+  >- (metis_tac[IN_FRANGE_DOMSUB_suff])
+  >- (res_tac >> irule term_ok'_extend >>
+      qexists_tac `<|tms := tms; tys := tys; axs := axs;
+                     etms := etms; etys := etys; eaxs := eaxs|>` >>
+      simp[ctys_def, ctms_def])
+  >- (res_tac >> irule term_ok'_extend >>
+      qexists_tac `<|tms := tms; tys := tys; axs := axs;
+                     etms := etms; etys := etys; eaxs := eaxs|>` >>
+      simp[ctys_def, ctms_def])
+QED
+
+Theorem theory_ok'_conservative_extend:
+  theory_ok' <|tms := tms; tys := tys; axs := axs; etms := etms; etys := etys; eaxs := eaxs|> ∧
+  tys ⊑ tys2 ∧ tms ⊑ tms2 ∧
+  DISJOINT (FDOM tys2) (FDOM etys) ∧
+  DISJOINT (FDOM tms2) (FDOM etms) ∧
+  (∀ty. ty ∈ FRANGE tms2 ⇒ type_ok tys2 ty) ∧
+  (∀p. p ∈ axs2 ⇒
+    term_ok' <|tms := tms2; tys := tys2; axs := axs2; etms := etms; etys := etys; eaxs := eaxs|> p ∧
+    p has_type Bool) ∧
+  is_std_sig (tys2, tms2) ∧
+  axioms_ok axs2 ⇒
+  theory_ok' <|tms := tms2; tys := tys2; axs := axs2; etms := etms; etys := etys; eaxs := eaxs|>
+Proof
+  strip_tac >>
+  `tys ⊌ etys ⊑ tys2 ⊌ etys ∧ tms ⊌ etms ⊑ tms2 ⊌ etms` by (
+    rw[SUBMAP_FLOOKUP_EQN, FLOOKUP_FUNION, AllCaseEqs()] >>
+    metis_tac[SUBMAP_FLOOKUP_EQN, IN_DISJOINT, FLOOKUP_DEF]
+  ) >>
+  gvs[theory_ok'_def, sigof'_def, ctys_def, ctms_def] >>
+  rpt conj_tac >> rpt strip_tac
+  >- (irule type_ok_extend >> qexists_tac `tys ⊌ etys` >> simp[] >> res_tac)
+  >- (rpt strip_tac >> res_tac >> irule term_ok'_extend >>
+      first_assum (irule_at (Pat `term_ok' _ _`)) >>
+      simp[ctys_def, ctms_def])
+QED
+
+Theorem updates_theory_ok':
+  upd updates' ctxt ⇒
+    theory_ok' (ethyof ctxt) ⇒ theory_ok' (ethyof (upd::ctxt))
+Proof
+  Induct_on `$updates'` >> rw[conexts_of_upd'_def]
+  (* NewAxiom: only axs changes, prop is CLOSED *)
+  >- (fs[theory_ok'_def, axioms_ok_def, CLOSED_def]
+      >> rpt conj_tac >> rpt strip_tac >> gvs[sigof'_def]
+      >> TRY (res_tac >> gvs[ctys_def, ctms_def])
+      >> irule (iffRL term_ok'_sig_eq)
+      >> qexists_tac `<|tms := tmsof ctxt; tys := tysof ctxt; axs := axsof' ctxt;
+                        etms := etmsof ctxt; etys := etysof ctxt; eaxs := eaxsof' ctxt|>`
+      >> simp[ctys_def, ctms_def]
+      >> res_tac >> simp[])
+  (* NewConst: tms gets a new entry *)
+  >- (irule theory_ok'_tms_extend >> simp[])
+  (* ConstSpec *)
+  >- (irule theory_ok'_conservative_extend >> cheat)
+  (* NewType: tys gets a new entry *)
+  >- (irule theory_ok'_tys_extend >> simp[])
+  (* TypeDefn *)
+  >- (irule theory_ok'_conservative_extend >> cheat)
+  (* NewEliminableType: only etys changes *)
+  >- (irule theory_ok'_etys_extend >> simp[])
+  (* NewEliminableConst: only etms changes *)
+  >- (irule theory_ok'_etms_extend >> simp[])
+  (* NewEliminableAxiom: only eaxs changes *)
+  >- (fs[theory_ok'_def, axioms_ok_def]
+      >> rpt conj_tac >> rpt strip_tac >> gvs[sigof'_def]
+      >> TRY (res_tac >> gvs[ctys_def, ctms_def])
+      >> irule (iffRL term_ok'_sig_eq)
+      >> qexists_tac `<|tms := tmsof ctxt; tys := tysof ctxt; axs := axsof' ctxt;
+                        etms := etmsof ctxt; etys := etysof ctxt; eaxs := eaxsof' ctxt|>`
+      >> simp[ctys_def, ctms_def]
+      >> res_tac >> simp[])
+QED
+
+Theorem extends_theory_ok':
+  ctxt2 extends' ctxt1 ⇒ theory_ok' (ethyof ctxt1) ⇒ theory_ok' (ethyof ctxt2)
+Proof
+  MATCH_MP_TAC (SPEC ``\x:update' list. theory_ok' (ethyof x)`` extends'_ind |> SIMP_RULE std_ss []) >>
+  metis_tac[updates_theory_ok']
 QED
 
 
